playgrounds/ioss.lean
@@ -1,0 +1,76 @@
+def bufsize : USize := 20 * 1024
+
+partial def dump (stream : IO.FS.Stream) : IO Unit := do
+  let buf ← stream.read bufsize
+  if buf.isEmpty then
+    pure ()
+  else
+    let stdout ← IO.getStdout
+    stdout.write buf
+    dump stream
+
+def fileStream (filename : System.FilePath) : IO (Option IO.FS.Stream) := do
+  let fileExists ← filename.pathExists
+  if not fileExists then
+    let stderr ← IO.getStderr
+    stderr.putStrLn s!"File not found: {filename}"
+    pure none
+  else
+    let handle ← IO.FS.Handle.mk filename IO.FS.Mode.read
+    pure $ some $ IO.FS.Stream.ofHandle handle
+
+
+def docString :=
+    "
+
+    feline
+
+    Print and concatenate files.
+    More information: <https://lean-lang.org/functional_programming_in_lean/hello-world/cat.html>.
+
+    - Print the contents of a file to `stdout`:
+        feline path/to/file
+
+    - Print several files to `stdout`:
+        feline path/to/file1 path/to/file2 ...
+
+    - Print the `stdin` alternating with files:
+        echo 'example' | feline path/to/file1 - path/to/file2
+
+    "
+
+def writeDoc : IO Unit := do
+  let stdout ← IO.getStdout
+  stdout.putStrLn docString
+
+
+def process (exitCode : UInt32) (args : List String) : IO UInt32 := do
+
+match args with
+  | []               => pure exitCode
+  | "-" :: args      =>
+    let stdin ← IO.getStdin
+    dump stdin
+    process exitCode args
+  | "--help" :: args =>
+    writeDoc
+    process exitCode args
+  | filename :: args =>
+    let stream ← fileStream ⟨filename⟩
+    match stream with
+    | none =>
+      process 1 args
+    | some stream =>
+      dump stream
+      process exitCode args
+
+
+def main (args : List String) : IO UInt32 :=
+  match args with
+  | [] => process 0 ["-"]
+  | _  =>  process 0 args
+
+def pegar_numero : IO Int := do
+  let stdin  ← IO.getStdin
+  let stdout ← IO.getStdout
+  let input  ← stdin.getLine
