playgrounds/playground-monad2.lean
@@ -19,30 +19,25 @@ open Arith in
 def fourteenDivided : Expr Arith :=
   prim div (const 14) (prim minus (const 45) (prim times (const 5) (const 9)))
 
-def applyPrimOption : Arith → Int → Int → Option Int
-  | Arith.plus, x, y => pure (x + y)
-  | Arith.minus, x, y => pure (x - y)
-  | Arith.times, x, y => pure (x * y)
-  | Arith.div, x, y =>
+def applyDivOption (x : Int) (y : Int) : Option Int :=
     if y == 0 then
       none
     else pure (x / y)
 
-def applyPrimExcept : Arith → Int → Int → Except String Int
-  | Arith.plus, x, y => pure (x + y)
-  | Arith.minus, x, y => pure (x - y)
-  | Arith.times, x, y => pure (x * y)
-  | Arith.div, x, y =>
+def applyDivExcept (x : Int) (y : Int) : Except String Int :=
     if y == 0 then
       Except.error s!"Tried to divide {x} by zero"
     else pure (x / y)
 
-def evaluateM [Monad m] (applyPrim : Arith → Int → Int → m Int): Expr Arith → m Int
+def applyPrim [Monad m] (applyDiv : Int → Int → m Int) : Arith → Int → Int → m Int
+  | Arith.plus , x, y => pure (x + y)
+  | Arith.minus, x, y => pure (x - y)
+  | Arith.times, x, y => pure (x * y)
+  | Arith.div  , x, y => applyDiv x y
+
+def evaluateM [Monad m] (applyDiv : Int → Int → m Int): Expr Arith → m Int
   | Expr.const i => pure i
   | Expr.prim p e1 e2 =>
-    evaluateM applyPrim e1 >>= fun v1 =>
-    evaluateM applyPrim e2 >>= fun v2 =>
-    applyPrim p v1 v2
-
-#eval evaluateM applyPrimOption fourteenDivided
-#eval evaluateM applyPrimExcept fourteenDivided
+    evaluateM applyDiv e1 >>= fun v1 =>
+    evaluateM applyDiv e2 >>= fun v2 =>
+    applyPrim applyDiv p v1 v2
