playgrounds/playground-monad3.lean
@@ -1,0 +1,56 @@
+inductive Expr (op : Type) where
+  | const : Int → Expr op
+  | prim : op → Expr op → Expr op → Expr op
+
+inductive Prim (special : Type) where
+  | plus
+  | minus
+  | times
+  | other : special → Prim special
+
+inductive CanFail where
+  | div
+
+def divOption : CanFail → Int → Int → Option Int
+  | CanFail.div, x, y => if y == 0 then none else pure (x / y)
+
+def divExcept : CanFail → Int → Int → Except String Int
+  | CanFail.div, x, y =>
+    if y == 0 then
+      Except.error s!"Tried to divide {x} by zero"
+    else pure (x / y)
+
+def applyPrim [Monad m] (applySpecial : special → Int → Int → m Int) : Prim special → Int → Int → m Int
+  | Prim.plus, x, y => pure (x + y)
+  | Prim.minus, x, y => pure (x - y)
+  | Prim.times, x, y => pure (x * y)
+  | Prim.other op, x, y => applySpecial op x y
+
+def evaluateM [Monad m] (applySpecial : special → Int → Int → m Int): Expr (Prim special) → m Int
+  | Expr.const i => pure i
+  | Expr.prim p e1 e2 =>
+    evaluateM applySpecial e1 >>= fun v1 =>
+    evaluateM applySpecial e2 >>= fun v2 =>
+    applyPrim applySpecial p v1 v2
+
+inductive MyEmpty where
+
+open MyEmpty
+
+def void_function : Empty → Empty :=
+  fun e =>        nomatch e
+
+def isConst (f : α → β) := ∀(a a' : α), f a = f a'
+
+theorem void_func_const : isConst void_function := by
+  rw [isConst]
+  intro e
+  cases e
+
+theorem uni_void_func : ∀(f g : Empty → Empty), f = g  := by
+  intros f g
+  funext e
+  cases e
+
+def applyEmpty [Monad m] (op : Empty) (_ : Int) (_ : Int) : m Int :=
+  nomatch op
