playgrounds/t1.lean
@@ -1,0 +1,193 @@
+/- Define some constants. -/
+
+def m : Nat := 1       -- m is a natural number
+def n : Nat := 0
+def b1 : Bool := true  -- b1 is a Boolean
+def b2 : Bool := false
+
+/- Check their types. -/
+
+#check m            -- output: Nat
+#check n
+#check n + 0        -- Nat
+#check m * (n + 0)  -- Nat
+#check b1           -- Bool
+#check b1 && b2     -- "&&" is the Boolean and
+#check b1 || b2     -- Boolean or
+#check true         -- Boolean "true"
+
+/- Evaluate -/
+
+#eval 5 * 4         -- 20
+#eval m + 2         -- 3
+#eval b1 && b2      -- false
+
+#check Nat               -- Type
+#check Bool              -- Type
+#check Nat → Bool        -- Type
+#check Nat × Bool        -- Type
+#check Nat → Nat         -- ...
+#check Nat × Nat → Nat
+#check Nat → Nat → Nat
+#check Nat → (Nat → Nat)
+#check Nat → Nat → Bool
+#check (Nat → Nat) → Nat
+
+def α : Type := Nat
+def β : Type := Bool
+def G : Type → Type → Type := Prod
+
+#check α        -- Type
+#check G α      -- Type → Type
+#check G α β    -- Type
+#check G α Nat  -- Type
+
+
+#check Prod α β       -- Type
+#check α × β          -- Type
+
+#check Prod Nat Nat   -- Type
+#check Nat × Nat      -- Type
+#check Type     -- Type 1
+#check Type 1   -- Type 2
+#check Type 2   -- Type 3
+#check Type 3   -- Type 4
+#check Type 4   -- Type 5
+
+#check Prop
+#check trivial
+
+#check List    -- List.{u} (α : Type u) : Type u
+#check Prod    -- Prod.{u, v} (α : Type u) (β : Type v) : Type (max u v)
+
+def F'.{u} (α : Type u) : Type u := Prod α α
+
+def F (α : Type u) : Type u := Prod α α
+
+
+#check F    -- Type u → Type u
+
+variable (x y : Nat)
+variable (n : true)
+
+def compose (g : β → γ) (f : α → β) (x : α) : γ :=
+  g (f x)
+
+variable (α β γ : Type)
+def doTwice (h : α → α) (x : α) : α :=
+  h (h x)
+
+def doThrice (h : a → a) (x : a) : a :=
+  h (h (h x))
+
+#check Sigma.mk 3 4
+#check (3, 4)
+
+
+#check doThrice
+#eval doThrice (· + 1) 3
+
+-- def brincador (b : True) : Nat := 5
+
+universe u v
+
+def f (α : Type u) (β : α → Type v) (a : α) (b : β a) : (a : α) × β a :=
+  ⟨a, b⟩
+
+def g (α : Type u) (β : α → Type v) (a : α) (b : β a) : Σ a : α, β a :=
+  Sigma.mk a b
+
+def h0 (n : Nat) : List Nat :=
+  (f Type List Nat [n]).2
+
+def h02 (n : Nat) : Type :=
+  (f Type List Nat [n]).1
+
+#check h0
+#check h0 3
+#eval  h0 3
+
+def h1 (x : Nat) : Nat :=
+  (f Type (fun α => α) Nat x).2
+
+#eval h1 5 -- 5
+
+def h2 (x : Nat) : Nat :=
+  (g Type (fun α => α) Nat x).2
+
+#eval h2 5 -- 5
+
+section
+  variable {α : Type u}
+  variable (x : α)
+  def ident := x
+end
+
+#check ident
+#check ident 4
+#check ident "hello"
+
+#check id 3      --> Nat
+#check @id Int 3 --> Int
+
+#check "olamundo"
+#check (4 : Int)
+#check String
+#check Int
+#check Type
+
+open List
+
+-- def sum : List Int → Int
+--   := foldl (· + ·) 0
+
+-- def subsequences {α : Type} : List α → List (List α)
+--   | [] => [[]]
+--   | a :: as =>
+--     let ass := subsequences as
+--     ass.map (a :: ·) ++ ass
+
+-- version com max?
+def bigger := foldl max (0 : Int)
+
+def tails {α : Type} (as : List α) : List (List α) :=
+  match as with
+  | [] => [[]]
+  | _ :: as' => as :: tails as'
+
+#eval tails [1, 2, 3]
+
+def inits {α : Type} (as : List α) : List (List α) :=
+  match as with
+  | [] => []
+  | a :: as' => [a] :: (cons a <$> inits as')
+
+#eval inits [1, 2, 3]
+#eval inits [1, 2]
+#eval inits [3]
+
+#eval tails [1, 2, 3]
+#eval tails [1, 2]
+#eval tails [3]
+
+def subsequences {α : Type} : List α → List (List α) :=
+  flatten ∘ map inits ∘ tails
+
+
+#eval flatten (map inits $ tails [1, 2, 3] )
+def solution :=
+  bigger ∘ map sum ∘ subsequences
+
+#eval solution [-1, -4, 3, -2, 44, -40, 8, 9, 11, 10, 0, 0, -1]
+#eval solution [3, -2, 44, -40, 8, 9, 11, 10]
+
+#eval subsequences [1, 2, 3]
+#eval subsequences [1, 2]
+
+#eval sum [1, -4, 5, 8, -1, 9]
+#eval sum [-4 -1]
+#eval sum ([] : List Int)
+#eval sum [5, 8, -1]
+#eval sum [5, 8]
+#eval sum [1, -4, 5, 8]
+#eval sum [5, 8, -1, 9]
