playgrounds/t2.lean
@@ -1,0 +1,114 @@
+-- [1, 2, 3, 4]
+-- [5, 6, 7, 8]
+
+--     1  2  3  4
+-- 5  [6, 7, 8, 9]
+-- 6  [7, ...]
+-- 7  []
+-- 8  []
+
+section s1
+  open List
+
+  universe u
+  variable {α β γ : Type u}
+
+  def zip_matrix_with (op : α → β → γ) : List α → List β → List (List γ)
+    | []     , _  => []
+    | a :: as, bs => map (op a) bs :: zip_matrix_with op as bs
+
+  def count_matrix : List (List α) → Nat :=
+    sum ∘ map length
+
+  #eval zip_matrix_with (· ++ " " ++ ·) ["oi", "tchau"] ["mundo", "vida"]
+  #eval zip_matrix_with (· + ·) [1, 2, 3, 4] [6, 7, 8, 9]
+  #eval zip_matrix_with (·, ·) [1, 2, 3, 4] [6, 7, 8, 9]
+
+  #check length
+  #eval count_matrix $ zip_matrix_with (· + ·) [1, 2, 3, 4] [6, 7, 8, 9]
+  #eval count_matrix $ zip_matrix_with (·, ·) [1, 2, 3, 4] [6, 7, 8, 9]
+
+  theorem T1 : ∀(xs : List α), ∀(ys : List β), ∀(op : α → β → γ),
+   count_matrix (zip_matrix_with op xs ys) = xs.length * ys.length := by
+
+  intros xs ys
+  intro op
+  induction xs with
+    | nil =>
+      rw [zip_matrix_with]
+      simp
+      rw [count_matrix]
+      simp
+
+    | cons x xs' hi =>
+      -- simp [zip_matrix_with, count_matrix, hi]
+      rw [length]
+      rw [Nat.succ_mul]
+      rw [<- hi]
+      rw [zip_matrix_with]
+      rw [count_matrix]
+      simp
+      rw [Nat.add_comm]
+
+  #check get?
+  #check bind
+
+  def l₁ := [1, 2, 3, 4, 5]
+  def l₂ := [9, 8, 7, 6, 5]
+
+  def m := zip_matrix_with (·, ·) l₁ l₂
+  
+  #eval m
+  #eval get? m 0
+  #check get? m 0
+end s1
+
+open List (get?)
+
+#eval m
+#eval get? m 0
+#check get? m 0
+#check bind (get? m 0)
+#check (get? m 0) >>= (flip get? 0)
+#check flip get?
+#check m.get? 0
+-- m a := Option <List natxnat>
+-- a -> m b := List <nat x nat> -> Optional <nat x nat>
+
+#check ((get? l₁ 0), (get? l₂ 0))
+
+def no_name : (Option α × Option β) → Option (α × β)
+  | (some a, some b) => some (a, b)
+  | _ => none
+
+def uncurry : (α → β → γ) → (α × β → γ)
+  | f, (a, b) => f a b
+
+#check no_name ((get? l₁ 0), (get? l₂ 0))
+
+theorem correctness : ∀(xs : List α), ∀(ys : List β), ∀(op : α → β → γ), ∀(n m : Nat),
+  -- ∀(n m : Nat), n < xs.length ∧ m < ys.length →
+  (get? (zip_matrix_with op xs ys) n) >>= (flip get? m)
+    = no_name ((get? xs n), (get? ys m)) >>= some ∘ uncurry op := by
+
+  intros xs ys op
+  intros n m
+  sorry
+
+
+def x     := 3 + 4 + 5
+def f x y := x + y + 4
+
+#check f
+
+#check Prop
+
+#check "oi"
+#check String
+#check Type
+
+def endoF (α : Type) : Type :=
+  α → α
+
+def idd : endoF Nat
+  | n => n
