playgrounds/t3.lean
@@ -1,0 +1,408 @@
+-- Functor -> Applicatives -> Monads
+namespace show_case
+  def divides x y := ∃ (k : Nat), x * k = y
+  infix:1000 "|" => divides
+  -- infix:500 "&"  => And
+  -- infix:500 "ou" => Or
+  -- notation x"|"y => divides x y
+
+  theorem div_trans : ∀ (x y z : Nat), x|y ∧ y|z → x|z := by
+  intros a b c
+  intro h
+  let h₁ := And.left h
+  let h₂ := And.right h
+  obtain ⟨k, hk⟩ := h₁
+  obtain ⟨q, hq⟩ := h₂
+  rw [divides]
+  exists (k * q)
+  rw [← Nat.mul_assoc]
+  rw [hk]
+  exact hq
+
+end show_case
+
+def kurry (f : α × β × γ → δ) : (α → β → γ → δ) :=
+  fun a b g => f (a, (b, g))
+
+def curry : (α × β → γ) → α → β → γ :=
+  fun f x y => f (x, y)
+
+def uncurry : (α → β → γ) → α × β → γ :=
+  fun f (x, y) => f x y
+
+def flipp (f : α → β → γ) : β → α → γ :=
+  fun b a => f a b
+
+section test
+variable {α β γ δ : Type}
+#check (α × (β × γ)) → δ
+
+def pog : (Nat × Int × Float) → Nat :=
+  fun (m, _, _) => m
+
+#check fun n => curry $ (curry pog) n
+#check fun n => curry $ (curry pog) n
+#check (kurry) (pog )
+#check ((curry ∘ ·) ∘ curry) pog
+
+def pogg : (Char × Nat × Int × Float) → Nat :=
+  fun (_, m, _, _) => m
+
+#check fun n => curry $ (curry pogg) n
+#check fun (n, m) => curry $ (fun n => curry $ (curry pogg) n) n m
+#check fun (n, m) => curry $ (fun n => curry $ (curry pogg) n) n m
+
+#check (((curry ∘ ·) ∘ curry ∘ ·) ∘ curry) pogg
+#check ((curry ∘ ·) ∘ curry) pog
+
+#check absurd -- absurd.{v} {a : Prop} {b : Sort v} (h₁ : a) (h₂ : ¬a) : b
+
+end test
+
+
+
+
+
+-- (A × B × C → D) → A → B → C → D
+#eval 3
+#check 3
+#check some 3
+#check (none : Option Nat)
+
+def tres_embalado := some 3
+def codigo_cliente : Option Int := none
+
+#check tres_embalado
+#check codigo_cliente
+
+
+def maybe_div2 (n : Nat) : Option Nat :=
+  if n % 2 = 0 then
+    some (n / 2)
+  else
+    none
+
+-- pure : α → m α
+-- bind : m α × (α → m β) → m β
+
+#check (· + 2)
+
+#eval ((pure  ∘ (· + 2)) 4 : Option Nat)
+
+#eval maybe_div2 5
+#eval bind (maybe_div2 20) maybe_div2
+#eval (maybe_div2 56)
+#eval bind (bind (maybe_div2 56) maybe_div2) maybe_div2
+#eval bind (bind (bind (maybe_div2 112) maybe_div2) maybe_div2) maybe_div2
+#eval maybe_div2 112 >>= maybe_div2
+                     >>= maybe_div2
+
+#eval maybe_div2 =<< maybe_div2 56
+
+#eval maybe_div2 112 >>= maybe_div2
+                     >>= pure ∘ (· + 2)
+                     >>= pure ∘ (· * 2)
+                     >>= maybe_div2
+                     >>= maybe_div2
+
+
+#eval maybe_div2 112 >>= maybe_div2
+                     >>= maybe_div2 ∘ (· * 2) ∘ (· + 2)
+                     >>= maybe_div2
+
+#eval maybe_div2 112 >>= pure ∘ (· + 2)
+                     >>= maybe_div2
+
+#eval do {
+  let x <- maybe_div2 112;
+  let y <- maybe_div2 (x + 2);
+  return y
+}
+
+-- def lesses (n : Nat) : List Nat :=
+--   match n with
+--   | 0     => []
+--   | k + 1 => k :: lesses k
+
+-- #eval lesses 5
+-- #eval lesses 15
+
+inductive Result
+
+-- def rust : IO Nat := do {
+--   let exit := return 0
+--   let opt_x <- pure (maybe_div2 38)
+--   match opt_x with
+--   | none   => exit
+--   | some x =>
+--     let opt_y <- pure (maybe_div2 x)
+--       match opt_y with
+--       | none   => exit
+--       | some y =>
+--         let opt_z <- pure (maybe_div2 y)
+--           match opt_z with
+--           | none   => exit
+--           | some z => pure z
+-- }
+
+-- #print rust
+
+-- #eval rust
+
+
+-- pure : α → m α
+-- bind : m α → (α → m β) → m β
+--
+
+def Implies (p q : Prop) : Prop := p → q
+  #check And     -- Prop → Prop → Prop
+  #check Or      -- Prop → Prop → Prop
+  #check Not     -- Prop → Prop
+  #check Implies -- Prop → Prop → Prop
+
+  variable (p q r : Prop)
+  #check And p q                      -- Prop
+  #check Or (And p q) r               -- Prop
+  #check Implies (And p q) (And q p)  -- Prop
+  #check Prop
+
+variable (p q : Prop)
+
+structure Proof (p : Prop) : Type where
+  proof : p
+
+#check Proof   -- Proof : Prop → Type
+
+axiom and_commm (p q : Prop) : Proof (Implies (And p q) (And q p))
+
+#check and_commm p q     -- Proof (Implies (And p q) (And q p))
+
+axiom modus_ponens  : (p q : Prop) → Proof (Implies p q) → Proof p → Proof q
+axiom implies_intro : (p q : Prop) → (Proof p → Proof q) → Proof (Implies p q)
+
+#check Sort 0 → Sort 0
+#check p → q
+#check Nat
+#check String
+#check Nat → String
+#check Sort 1
+
+namespace working_with_propositions_as_types
+
+variable {p q : Prop}
+
+theorem t1_0 : p → q → p :=
+  fun hp : p =>
+    (fun hq : q =>
+      hp)
+
+theorem t1_1 : p → q → p :=
+  fun hp : p =>
+    fun _ => hp
+
+
+def t1_2 : p → q → p :=
+  fun hp : p =>
+    fun _ => hp
+
+#print t1_2
+#print t1_1
+#print t1_0
+
+theorem t1_3 : p → q → p :=
+  fun hp : p =>
+  fun hq : q =>
+  show p from hp
+
+#print t1_3
+
+theorem t1_4 (hp : p) (hq : q) : p := hp
+
+axiom hp : p
+
+theorem t2 : q → p := t1_4 hp
+
+#print t1_4
+
+axiom u       : Empty
+axiom unsound : False
+
+#check False
+#eval  False
+#print False
+#print True
+
+-- Everything follows from false (- in some worlds)
+
+theorem ex : 1 = 0 :=
+  False.elim unsound
+
+#print ex
+
+
+theorem t1_5 {p q : Prop} (hp : p) (hq : q) : p := hp
+
+#print t1_5
+
+theorem t1_6 : ∀ {p q : Prop}, p → q → p :=
+  fun {p q : Prop} (hp : p) (hq : q) => hp
+
+#print t1_6
+
+def id_0 {α : Type} : α → α :=
+  id
+
+def id_1 : ∀ {α : Type}, α → α :=
+  id
+
+variable (hp : p)
+
+theorem t1_7 : q → p :=
+  fun _ =>
+    show p from hp
+
+#print t1_6
+#check t1_6
+
+section s1
+  theorem t1 (p q : Prop) (hp : p) (hq : q) : p := hp
+
+  variable (p q r s : Prop)
+
+  #check t1 p q                -- p → q → p
+  #check t1 r s                -- r → s → r
+  #check t1 (r → s) (s → r)    -- (r → s) → (s → r) → r → s
+
+  variable (h : r → s)
+  #check t1 (r → s) (s → r) h  -- (s → r) → r → s
+end s1
+
+section s2
+  variable (p q r s : Prop)
+
+  theorem t2_0 (h₁ : q → r) (h₂ : p → q) : p → r :=
+    fun hₚ : p =>
+    show r from (h₁ ∘ h₂) hₚ
+end s2
+
+
+end working_with_propositions_as_types
+
+namespace testing_more
+variable (p q : Prop)
+
+example (hp : p) (hq : q) : p ∧ q := And.intro hp hq
+
+#check fun (hp : p) (hq : q) => And.intro hp hq
+
+#check And.intro -- {a b : Prop} (left : a) (right : b) : a ∧ b
+#check And.left  -- {a b : Prop} (self : a ∧ b) : a
+#check And.right -- {a b : Prop} (self : a ∧ b) : b
+
+example (h : p ∧ q) : q ∧ p :=
+  show q ∧ p from ⟨h.right, h.left⟩
+
+end testing_more
+
+namespace disjuction
+variable (p q : Prop)
+example (hp : p) : p ∨ q := Or.intro_left q hp
+example (hq : q) : p ∨ q := Or.intro_right p hq
+
+#check Or.intro_left  -- {a : Prop} (b : Prop) (h : a) : a ∨ b
+#check Or.intro_right -- {b : Prop} (a : Prop) (h : b) : a ∨ b
+#check Or.elim        -- {a b c : Prop} (h : a ∨ b) (left : a → c) (right : b → c) : c
+#check Or.inl         -- {a b : Prop} (h : a) : a ∨ b
+#check Or.inr         -- {a b : Prop} (h : a) : a ∨ b
+
+
+
+example (h : p ∨ q) : q ∨ p :=
+  Or.elim h
+    (fun hp : p =>
+      show q ∨ p from Or.intro_right q hp)
+    (fun hq : q =>
+      show q ∨ p from Or.intro_left p hq)
+
+example (h : p ∨ q) : q ∨ p :=
+  h.elim (fun hp => Or.inr hp) (fun hq => Or.inl hq)
+
+end disjuction
+
+namespace negation
+variable (p q : Prop)
+example (hpq : p → q) (hnq : ¬q) : ¬p :=
+  fun hp : p =>
+  show False from hnq (hpq hp)
+
+example (hp : p) (hnp : ¬p) : q := False.elim (hnp hp)
+
+#check False.elim -- False.elim.{u} {C : sort u} (h : False) : C
+
+variable (p q r : Prop)
+
+example (hnp : ¬p) (hq : q) (hqp : q → p) : r :=
+  absurd (hqp hq) hnp
+
+#check True.intro
+
+end negation
+
+namespace iff
+
+variable {p q : Prop}
+#check Iff.intro -- {a b : Prop} (mp : a → b) (mpr : b → a) : a ↔ b
+def thing : p ↔ p := ⟨id , id⟩
+#check Iff.intro -- {a b : Prop} (mp : a → b) (mpr : b → a) : a ↔ b
+#check Iff.mp    -- {a b : Prop} (self : a ↔ b) : a → b
+#check Iff.mpr   -- {a b : Prop} (self : a ↔ b) : b → a
+
+variable (p q : Prop)
+
+theorem and_swap : p ∧ q ↔ q ∧ p :=
+  let f {r s : Prop} (h : r ∧ s) : s ∧ r := ⟨h.2, h.1⟩
+  ⟨f, f⟩
+
+example (h : p ∧ q) : q ∧ p := (and_swap p q).mp h
+
+end iff
+
+namespace subgoals
+variable (p q : Prop)
+
+example (h : p ∧ q) : q ∧ p :=
+  have hp : p := h.left
+  have hq : q := h.right
+  show q ∧ p from ⟨hq, hp⟩
+
+example (h : p ∧ q) : q ∧ p :=
+  let hp : p := h.left
+  let hq : q := h.right
+  show q ∧ p from ⟨hq, hp⟩
+
+variable (p q : Prop)
+
+example (h : p ∧ q) : q ∧ p :=
+  have hp : p := h.left
+  suffices hq : q from And.intro hq hp
+  show q from And.right h
+
+end subgoals
+
+namespace classical
+open Classical
+
+variable (p : Prop)
+
+#check em              -- Classical.em (p : Prop) : p ∨ ¬p
+#check byCases         -- {p q : Prop} (hpq : p → q) (¬p → q) : q
+#check byContradiction -- {p : Prop} (h : ¬p → False) : p
+#check Classical.em
+
+
+theorem dne {p : Prop} (h : ¬¬p) : p :=
+  Or.elim (em p)
+    (fun hp : p => hp)
+    (fun hnp : ¬p => absurd hnp h)
+
+end classical
