programs/compiler_test01/evaluator.lean
@@ -1,0 +1,69 @@
+
+inductive Tipe : Type 1 where
+| n
+| z
+| f
+| s
+| c
+| t
+
+def Op (α : Type) (ar : Nat) := List α → α
+
+#eval 3
+
+inductive SyntaxTree where
+| leaf   (t : Tipe) : SyntaxTree
+| branch (l : List SyntaxTree) : Op α ar → l.length = ar → SyntaxTree
+#check List.all
+
+def typecheck : SyntaxTree → Type :=
+  sorry
+
+def eval : SyntaxTree → α :=
+  sorry
+
+-- open Operator
+-- open SyntaxTree
+
+-- def ex0 := branch (leaf 3) times (leaf 4)
+-- def ex1 := branch (leaf 3) plus (leaf 4)
+-- def ex2 := branch ex1 times (leaf 5)
+-- def ex3 := branch ex1 times ex2
+-- def ex4 := branch ex0 times ex2
+
+-- def eval_string : SyntaxTree → String
+--   | leaf n        => toString n
+--   | branch l op r =>
+--   let par (str : String) := s!"({str})"
+--   par (match op with
+--   | plus  => (eval_string l) ++ " plus "  ++ (eval_string r)
+--   | times => (eval_string l) ++ " times " ++ (eval_string r))
+
+-- def eval_times : SyntaxTree → SyntaxTree
+--   | leaf n           => leaf n
+--   | branch l plus r  => branch (eval_times l) plus (eval_times r)
+--   | branch l times r =>
+--     let (l', r') := (eval_times l, eval_times r)
+--     match l', r' with
+--     | leaf n, leaf m => leaf (n * m)
+--     | _     , _      => branch l' times r'
+
+-- #eval eval_string ex3
+-- #eval eval_string ex4
+-- #eval eval_string (eval_times ex4)
+
+---------------------------------------------------------------------------------------------------------------------------
+
+inductive Foo : Type → Type 1 where
+| numb : Int  → Foo Int
+| bool : Bool → Foo Bool
+| plus : Foo Int  → Foo Int → Foo Int
+| not  : Foo Bool → Foo Bool
+| ite  : Foo Bool → Foo α → Foo α → Foo α
+deriving Repr
+
+open Foo
+
+#eval  numb 3
+#eval  ite (bool true) (numb 3) (numb 4)
+#check numb 3
